F_mu_ref_par/fundamental_unary.v
@@ -1,0 +1,240 @@
+Require Import iris.program_logic.hoare.
+Require Import iris.program_logic.lifting.
+Require Import iris.algebra.upred_big_op.
+Require Import F_mu_ref_par.lang F_mu_ref_par.typing F_mu_ref_par.rules
+        F_mu_ref_par.logrel_unary.
+From iris.program_logic Require Export lifting.
+From iris.algebra Require Import upred_big_op frac dec_agree.
+From iris.program_logic Require Export invariants ghost_ownership.
+From iris.program_logic Require Import ownership auth.
+Require Import iris.proofmode.tactics iris.proofmode.invariants.
+Import uPred.
+
+Section typed_interp.
+  Context {Σ : gFunctors} `{i : heapIG Σ} `{L : namespace}.
+
+  Implicit Types P Q R : iPropG lang Σ.
+  Notation "# v" := (of_val v) (at level 20).
+
+  Local Hint Extern 1 =>
+  match goal with
+    |-
+    (_
+       --------------------------------------□
+       ∃ _ : ?A, _) => let W := fresh "W" in evar (W : A); iExists W; unfold W; clear W
+  end : itauto.
+
+  Local Hint Extern 1 =>
+  match goal with
+    |-
+    (_
+       --------------------------------------□
+       ▷ _) => iNext
+  end : itauto.
+
+  Local Hint Extern 1 =>
+  match goal with
+    |-
+    (_
+       --------------------------------------□
+       □ _) => eapply (@always_intro _ _ _ _)
+  end : itauto.
+
+  Local Hint Extern 1 =>
+  match goal with
+    |-
+    (_
+       --------------------------------------□
+       (_ ∧ _)) => iSplit
+  end : itauto.
+
+  Local Tactic Notation "smart_wp_bind" uconstr(ctx) ident(v) constr(Hv) uconstr(Hp) :=
+    iApply (@wp_bind _ _ _ [ctx]);
+    iApply wp_impl_l;
+    iSplit; [| iApply Hp; trivial];
+    [apply (always_intro _ _); iIntros {v} Hv|iSplit; trivial]; cbn.
+
+  Local Ltac value_case := iApply wp_value; [cbn; rewrite ?to_of_val; trivial|].
+
+  Lemma typed_interp N Δ Γ vs e τ
+        (HNLdisj : ∀ l : loc, N ⊥ L .@ l)
+        (Htyped : typed Γ e τ)
+        (HΔ : context_interp_Persistent Δ)
+    : List.length Γ = List.length vs →
+      (heapI_ctx N ∧ Π∧ zip_with (λ τ v, (@interp Σ i L) τ Δ v) Γ vs)%I ⊢
+                  WP (e.[env_subst vs]) @ ⊤ {{ λ v, (@interp Σ i L) τ Δ v }}.
+  Proof.
+    revert Δ HΔ vs.
+    induction Htyped; intros Δ HΔ vs Hlen; iIntros "#[Hheap HΓ]"; cbn.
+    - (* var *)
+      destruct (lookup_lt_is_Some_2 vs x) as [v Hv].
+      { by rewrite -Hlen; apply lookup_lt_Some with τ. }
+      rewrite /env_subst Hv; value_case.
+      iApply (big_and_elem_of with "HΓ").
+      apply elem_of_list_lookup_2 with x.
+      rewrite lookup_zip_with; simplify_option_eq; trivial.
+    - (* unit *) value_case; trivial.
+    - (* pair *)
+      smart_wp_bind (PairLCtx e2.[env_subst vs]) v "#Hv" IHHtyped1.
+      smart_wp_bind (PairRCtx v) v' "# Hv'" IHHtyped2.
+      value_case; eauto 10 with itauto.
+    - (* fst *)
+      smart_wp_bind (FstCtx) v "# Hv" IHHtyped; cbn.
+      iApply double_exists; [|trivial].
+      intros w w'; cbn; iIntros "#[% [H2 H3]]"; rewrite H; cbn.
+      iApply wp_fst; eauto using to_of_val; cbn.
+    - (* snd *)
+      smart_wp_bind (SndCtx) v "# Hv" IHHtyped; cbn.
+      iApply double_exists; [|trivial].
+      intros w w'; cbn; iIntros "#[% [H2 H3]]"; rewrite H; cbn.
+      iApply wp_snd; eauto using to_of_val; cbn.
+    - (* injl *)
+      smart_wp_bind (InjLCtx) v "# Hv" IHHtyped; cbn.
+      value_case; iLeft; auto with itauto.
+    - (* injr *)
+      smart_wp_bind (InjRCtx) v "# Hv" IHHtyped; cbn.
+      value_case; iRight; auto with itauto.
+    - (* case *)
+      smart_wp_bind (CaseCtx _ _) v "#Hv" IHHtyped1; cbn.
+      iDestruct "Hv" as "[Hv|Hv]";
+      iDestruct "Hv" as {w} "[% Hw]"; rewrite H;
+        [iApply wp_case_inl|iApply wp_case_inr];
+        auto 1 using to_of_val;
+        asimpl;
+        [specialize (IHHtyped2 Δ HΔ (w::vs)) |
+         specialize (IHHtyped3 Δ HΔ (w::vs))];
+        erewrite <- ?typed_subst_head_simpl in * by (cbn; eauto); iNext;
+          [iApply IHHtyped2 | iApply IHHtyped3]; cbn; auto with itauto.
+    - (* lam *)
+      value_case; apply (always_intro _ _); iIntros {w} "#Hw".
+      iApply wp_lam; auto 1 using to_of_val.
+      asimpl; erewrite typed_subst_head_simpl; [|eauto|cbn]; eauto.
+      iNext; iApply (IHHtyped Δ HΔ (w :: vs)); cbn; auto with itauto.
+    - (* app *)
+      smart_wp_bind (AppLCtx (e2.[env_subst vs])) v "#Hv" IHHtyped1.
+      smart_wp_bind (AppRCtx v) w "#Hw" IHHtyped2.
+      iApply wp_mono; [|iApply "Hv"]; auto with itauto.
+    - (* TLam *)
+      value_case; iApply exist_intro; iSplit; trivial.
+      iIntros {τi}; destruct τi as [τi τiPr].
+      iRevert "Hheap".
+      iPoseProof (always_intro with "HΓ") as "HP"; try typeclasses eauto;
+        try (iApply always_impl; iExact "HP").
+      iIntros "#HΓ #Hheap"; iNext.
+      iApply IHHtyped; [rewrite map_length|]; trivial.
+      iSplit; trivial.
+      iRevert "Hheap HΓ". rewrite zip_with_context_interp_subst.
+      iIntros "#Hheap #HΓ"; trivial.
+    - (* TApp *)
+      smart_wp_bind TAppCtx v "#Hv" IHHtyped; cbn.
+      iDestruct "Hv" as {e'} "[% He']"; rewrite H.
+      iApply wp_TLam.
+      iSpecialize ("He'" $! ((interp τ' Δ) ↾ _)); cbn.
+      iApply always_elim. iApply always_mono; [|trivial].
+      iIntros "He'"; iNext.
+      iApply wp_mono; [|trivial].
+      iIntros {w} "#H". rewrite -interp_subst; trivial.
+    - (* Fold *)
+      rewrite map_length in IHHtyped.
+      iApply (@wp_bind _ _ _ [FoldCtx]).
+        iApply wp_impl_l.
+        iSplit; [eapply (@always_intro _ _ _ _)|
+                 iApply (IHHtyped (extend_context_interp ((interp (TRec τ)) Δ) Δ));
+                 trivial].
+      + iIntros {v} "#Hv".
+        value_case.
+        rewrite fixpoint_unfold; cbn.
+        auto with itauto.
+      + iRevert "Hheap HΓ"; rewrite zip_with_context_interp_subst;
+          iIntros "#Hheap #HΓ"; auto with itauto.
+    - (* Unfold *)
+      iApply (@wp_bind _ _ _ [UnfoldCtx]);
+        iApply wp_impl_l;
+        iSplit; [eapply (@always_intro _ _ _ _)|
+                 iApply IHHtyped;
+                 auto with itauto].
+      iIntros {v}.
+      cbn [interp interp_rec cofe_mor_car].
+      rewrite fixpoint_unfold.
+      iIntros "#Hv"; cbn.
+      change (fixpoint _) with (@interp _ _ L (TRec τ) Δ).
+      iDestruct "Hv" as {w} "[% #Hw]"; rewrite H.
+      iApply wp_Fold; cbn; auto using to_of_val.
+      rewrite -interp_subst; auto with itauto.
+    - (* Fork *)
+      iApply wp_fork.
+      iNext; iSplitL; trivial.
+      iApply wp_impl_l.
+      iSplit; [|iApply IHHtyped]; trivial.
+      { iApply always_intro; trivial. iIntros "#Hheap % #Hv"; trivial. }
+      iSplit; trivial.
+    - (* Alloc *)
+      smart_wp_bind AllocCtx v "#Hv" IHHtyped; cbn. iClear "HΓ".
+      iApply wp_atomic; cbn; trivial; [rewrite to_of_val; auto|].
+      iPvsIntro.
+      iApply wp_alloc; auto 1 using to_of_val.
+      iFrame "Hheap". iNext.
+      iIntros {l} "Hl".
+      iPvs (inv_alloc _ with "[Hl]") as "HN";
+        [| | iPvsIntro; iExists _; iSplit; trivial].
+      trivial.
+      iNext; iExists _; iFrame "Hl"; trivial.
+    - (* Load *)
+      smart_wp_bind LoadCtx v "#Hv" IHHtyped; cbn. iClear "HΓ".
+      iRevert "Hheap". iApply exist_elim; [|iExact "Hv"].
+      iIntros {l} "[% #Hv] #Hheap"; rewrite H.
+      iApply wp_atomic; cbn; eauto using to_of_val.
+      iPvsIntro.
+      iInv (L .@ l) as {w} "[Hw1 #Hw2]".
+      iApply (wp_load _ _ _ 1); [|iFrame "Hheap"]; trivial.
+      specialize (HNLdisj l); set_solver_ndisj.
+      iFrame "Hw1". iNext.
+      iIntros "Hw1". iSplitL; trivial.
+      iNext; iExists _. iFrame "Hw1"; trivial.
+    - (* Store *)
+      smart_wp_bind (StoreLCtx _) v "#Hv" IHHtyped1; cbn.
+      smart_wp_bind (StoreRCtx _) w "#Hw" IHHtyped2; cbn. iClear "HΓ".
+      iRevert "Hheap Hw". iApply exist_elim; [|iExact "Hv"].
+      iIntros {l} "#[% Hl] #Hheap #Hw"; rewrite H.
+      iApply wp_atomic; cbn; [trivial| rewrite ?to_of_val; auto |].
+      iPvsIntro.
+      iInv (L .@ l) as {z} "[Hz1 #Hz2]".
+      eapply bool_decide_spec; eauto using to_of_val.
+      iApply (wp_store N); auto using to_of_val.
+      specialize (HNLdisj l); set_solver_ndisj.
+      iFrame "Hheap Hz1".
+      iNext.
+      iIntros "Hz1".
+      iSplitL; [|iPvsIntro; trivial].
+      iNext; iExists _. iFrame "Hz1"; trivial.
+    - (* CAS *)
+      smart_wp_bind (CasLCtx _ _) v1 "#Hv1" IHHtyped1; cbn.
+      smart_wp_bind (CasMCtx _ _) v2 "#Hv2" IHHtyped2; cbn.
+      smart_wp_bind (CasRCtx _ _) v3 "#Hv3" IHHtyped3; cbn. iClear "HΓ".
+      iDestruct "Hv1" as {l} "[% Hinv]"; subst.
+      iApply wp_atomic; cbn; eauto 10 using to_of_val.
+      iPvsIntro.
+      iInv (L .@ l) as {w} "[Hw1 #Hw2]"; [cbn; eauto 10 using to_of_val|].
+      destruct (val_dec_eq v2 w) as [|Hneq]; subst.
+      + iApply (wp_cas_suc N); eauto using to_of_val.
+        specialize (HNLdisj l); set_solver_ndisj.
+        iFrame "Hheap Hw1".
+        iNext. iIntros "Hw1".
+        iSplitL.
+        * iNext; iExists _; iSplitL; trivial.
+        * iPvsIntro. iLeft; iExists _; auto with itauto.
+      + iApply (wp_cas_fail N); eauto using to_of_val.
+        clear Hneq. specialize (HNLdisj l); set_solver_ndisj.
+        (* Weird that Hneq above makes set_solver_ndisj diverge or
+           take exceptionally long!?!? *)
+        iFrame "Hheap Hw1".
+        iNext. iIntros "Hw1".
+        iSplitL.
+        * iNext; iExists _; iSplitL; trivial.
+        * iPvsIntro. iRight; iExists _; auto with itauto.
+      (* unshelving *)
+      Unshelve.
+      cbn; typeclasses eauto.
+  Qed.
+
+End typed_interp.
